capabilities/code/big_step.v
@@ -1,0 +1,218 @@
+Set Warnings "-notation-overridden,-parsing".
+(*
+Author: Rodrigo Raya
+
+Following "The Semantics of Ownership and Borrowing in the Rust Programming Language" by Nienke Wessel.
+*)
+
+From Coq Require Import ZArith.Int.
+From Coq Require Import omega.Omega.
+From Coq Require Import Lists.List.
+From Coq Require Import Strings.String.
+From Coq Require Import Logic.FunctionalExtensionality.
+Require Import Capabilities.CustomTactics.
+
+Import ListNotations.
+
+Definition vname := string.
+
+Inductive zext :=
+| non_declared
+| not_assigned
+| val : Z -> zext.
+
+Declare Scope move_scope.
+Bind Scope move_scope with zext.
+Notation "-__u" := non_declared : move_scope.
+Notation "⊥" := not_assigned : move_scope.
+ 
+Inductive type :=
+| Int : type.
+
+Inductive expr :=
+| var : vname -> expr
+| integer : Z -> expr
+| add : expr -> expr -> expr.
+
+Inductive com :=
+| Skip : com
+| Seq : com -> com -> com
+| Bind : vname -> type -> com -> com
+| Assign : vname -> expr -> com.
+
+Bind Scope move_scope with com.
+Notation "c1 ;; c2" :=
+  (Seq c1 c2) (at level 60, right associativity) : move_scope.
+(*
+The notation emphasizes that a let statement in Rust:
+
+let x = e
+
+actually refers to a two step process:
+
+1. Variable x is declared.
+2. A value is assigned to the resource x owns.
+
+We instead write:
+
+let x in (x = e) 
+*)
+Notation "'LET' x ',' t 'IN' b" :=
+  (Bind x t b) (at level 50, left associativity) : move_scope.
+Notation "x ';=' e" :=
+  (Assign x e) (at level 50) : move_scope.
+
+Definition prog0 : com := Skip.
+
+(* Some variables to work with *)
+Definition X : string := "x".
+Definition Y : string := "y".
+Definition Z : string := "z".
+
+Definition prog1 : com := LET X , Int IN Skip.
+
+Definition prog2 : com :=
+  LET X , Int IN (X ;= (integer 0) ;;
+   LET Y , Int IN (Y ;= (var X) ;;
+    LET Z , Int IN (Z ;= (var Y)))).
+
+Definition state := vname -> zext.
+
+Definition abs_state (A:Type) := string -> A.
+
+Definition update {abs_value: Type} 
+  (s : abs_state abs_value) (x : string) (v : abs_value) :=
+  fun x' => if String.eqb x x' then v else s x'.
+
+Lemma update_eq : forall (s: state) (x1 x2: string) (v: zext),
+    x1 = x2 -> update s x1 v x2 = v.
+Proof. unfold update; repeat light || destruct_match || strings. Qed.
+
+Lemma update_refl : forall (s: state) (x: string) (v: zext),
+    update s x v x = v.
+Proof. repeat lights || rewrite update_eq. Qed.
+
+Lemma update_neq : forall (s: state) (x1 x2: string) (v: zext),
+    x1 <> x2 -> update s x1 v x2 = s x2.
+Proof. unfold update; repeat light || destruct_match || strings. Qed.
+
+Lemma update_com :
+  forall (x1 x2: string) (s: state) (v: zext),
+    update (update s x1 v) x2 v = update (update s x2 v) x1 v.
+Proof.
+  unfold update; repeat light || destruct_match ||
+         apply functional_extensionality.
+Qed.
+
+Definition update_list {abs_value: Type} 
+  (s : abs_state abs_value) (l : list string) (v : abs_value) :=
+  fold_left (fun (s': abs_state abs_value) (x: string)
+             => update s' x v) l s.
+
+Lemma update_to_list :
+  forall (x: string) (l: list vname) (s: state) (v: zext),
+    update_list (update s x v) l v = update (update_list s l v) x v.
+Proof.
+  induction l;
+    repeat clarify || rewrite update_com || rewrite_back_any.
+Qed.
+
+Lemma update_list_neq :
+  forall (l: list string) (s: state) (x: string) (v: zext),
+    not (In x l) -> update_list s l v x = s x.
+Proof.
+  induction l; repeat clarify || rewrite_any || rewrite update_neq. 
+Qed.
+
+Lemma update_list_eq :
+  forall (l: list string) (s: state) (x: string) (v: zext),
+    In x l -> update_list s l v x = v.
+Proof.
+  induction l;
+  repeat clarify || rewrite update_to_list || unfold update ||
+         rewrite String.eqb_refl.
+Qed.
+
+Fixpoint vars (e: expr): list string :=
+  match e with
+  | var vn => [vn]
+  | integer i => []
+  | add e__1 e__2 => vars (e__1) ++ vars(e__2)
+  end.
+
+Fixpoint aval (s : state) (e : expr): zext :=
+  match e with
+  | var vn => s vn
+  | integer i => val i
+  | add e__1 e__2 =>
+     match (aval s e__1, aval s e__2) with
+     | (val i, val j) => val (i + j)
+     | _ => non_declared
+     end
+  end.
+
+Reserved Notation "e '⟹__b' b" (at level 90, left associativity).
+
+Inductive big_step : com * state -> state -> Prop :=
+| BSkip (s: state) : (Skip, s) ⟹__b s
+| BSeq (s__1 s__2 s__3: state) (c__1 c__2: com) :
+    (c__1,s__1) ⟹__b s__2 -> (c__2,s__2) ⟹__b s__3 -> (c__1;;c__2,s__1) ⟹__b s__3
+| BLet (s s': state) (c : com) (x : vname) (t : type) :
+    (c,update s x ⊥) ⟹__b s' ->
+     (LET x , t IN c, s) ⟹__b (update s' x (s x))
+| BAssign (s: state) (e : expr) (x: string) :
+    aval s (var x) = ⊥ -> aval s e <> ⊥ -> aval s e <> -__u ->
+    (x ;= e, s) ⟹__b (update_list (update s x (aval s e)) (vars e) -__u)
+where "e '⟹__b' b" := (big_step e b) : move_scope.
+
+Open Scope move_scope.
+
+Theorem big_step_deterministic : forall (c: com) (s s__1 s__2 : state),
+    (c,s) ⟹__b s__1 -> (c,s) ⟹__b s__2 -> s__1 = s__2.
+Proof.
+  Ltac inductive P :=
+      match goal with
+      | [ IH: forall s s1 s2, P (?c1,s) s1 ->
+                         P (?c1,s) s2 ->
+                         s1 = s2,
+            H1: P (?c1,?s) ?s3,
+            H2:  P (?c1,?s) ?s4 |- _ ] =>
+        pose proof (IH s s3 s4 H1 H2)
+      end.
+  induction c;
+  repeat light || invert_pred big_step || inductive big_step.
+Qed.
+
+(*
+After execution, a program no longer has variables in memory.
+*)
+Theorem variable_allocation:
+  forall (c: com) (s s' : state) (y : string),
+    (c,s) ⟹__b s' -> aval s (var y) = -__u -> aval s' (var y) = -__u.
+Proof.
+  Ltac destruct_updates :=
+    match goal with
+    | [ |- context[update _ ?x _ ?y] ] =>
+      destruct (String.eqb x y) eqn: eq
+    | [ |- context[update_list _ ?l _ ?y] ] =>
+      destruct (in_dec string_dec y l)
+    end.
+
+  Ltac inductive_update :=
+    repeat light || rewrite update_refl || rewrite update_neq ||
+           eapply_any.
+
+  Ltac inductive_update_list :=
+    match goal with
+    | [ H: In ?y ?l |- context[update_list _ ?l _ ?y] ] =>
+      rewrite update_list_eq; try light
+    | _ =>
+      rewrite update_list_neq; try light;
+      destruct_updates; inductive_update
+    end. 
+     
+  induction c;
+    repeat clarify || invert_pred big_step.
+  - destruct_updates; strings; inductive_update.
+  - destruct_updates; inductive_update_list.
+Qed.
