emacs
@@ -1,0 +1,19 @@
+find word in file
+
+https://www.gnu.org/software/emacs/manual/html_node/emacs/Word-Search.html
+
+Interrupt proving process (proof general):
+
+C-c C-c
+
+Browse definition:
+
+Cursor over definition and C - c C - d
+
+Change file:
+
+C-x b
+
+Remove other window different from current:
+
+C-x 1
